progs/ghostsI.v
@@ -17,8 +17,6 @@ Proof.
   exact own_alloc_strong.
 Qed.
 
-Set Printing All.
-
 Lemma own_alloc : forall (a : G) (pp : preds), valid a -> emp%I |-- (|==> EX g : own.gname, own g a pp)%I.
 Proof.
   exact own_alloc.
@@ -29,7 +27,7 @@ Proof.
   exact own_dealloc.
 Qed.
 
-Lemma own_update : forall g a b pp, fp_update a b -> (own g a pp |-- |==> own g b pp)%I.
+Lemma own_update : forall g a b pp, fp_update a b -> own g a pp |-- (|==> own g b pp)%I.
 Proof.
   exact own_update.
 Qed.
@@ -40,27 +38,27 @@ Proof.
 Qed.
 
 Lemma own_list_alloc : forall la lp, Forall valid la -> length lp = length la ->
-  (emp |-- |==> (EX lg : _, !!(Zlength lg = Zlength la) &&
+  emp |-- (|==> (EX lg : _, !!(Zlength lg = Zlength la) &&
     iter_sepcon (fun '(g, a, p) => own g a p) (combine (combine lg la) lp)))%I.
 Proof.
   exact own_list_alloc.
 Qed.
 
 Corollary own_list_alloc' : forall a pp i, 0 <= i -> valid a ->
-  (emp |-- |==> (EX lg : _, !!(Zlength lg = i) && iter_sepcon (fun g => own g a pp) lg))%I.
+  emp |-- (|==> (EX lg : _, !!(Zlength lg = i) && iter_sepcon (fun g => own g a pp) lg))%I.
 Proof.
   exact own_list_alloc'.
 Qed.
 
 Lemma own_list_dealloc : forall {A} f (l : list A),
   (forall b, exists g a pp, f b |-- own g a pp) ->
-  (iter_sepcon f l |-- |==> emp)%I.
+  iter_sepcon f l |-- (|==> emp)%I.
 Proof.
   intros; apply own_list_dealloc; auto.
 Qed.
 
 Lemma own_list_dealloc' : forall {A} g a p (l : list A),
-  (iter_sepcon (fun x => own (g x) (a x) (p x)) l |-- |==> emp)%I.
+  iter_sepcon (fun x => own (g x) (a x) (p x)) l |-- (|==> emp)%I.
 Proof.
   intros; apply own_list_dealloc'.
 Qed.
@@ -72,7 +70,7 @@ Qed.*)
 
 End ghost.
 
-Lemma exclusive_update : forall {A} (v v' : A) p, (excl p v |-- |==> excl p v')%I.
+Lemma exclusive_update : forall {A} (v v' : A) p, excl p v |-- (|==> excl p v')%I.
 Proof.
   intros; apply exclusive_update.
 Qed.
@@ -96,13 +94,13 @@ Proof.
   exact ghost_snap_forget.
 Qed.
 
-Lemma ghost_snap_choose : forall v1 v2 p, (ghost_snap v1 p * ghost_snap v2 p |-- |==> ghost_snap v1 p)%I.
+Lemma ghost_snap_choose : forall v1 v2 p, ghost_snap v1 p * ghost_snap v2 p |-- (|==> ghost_snap v1 p)%I.
 Proof.
   exact ghost_snap_choose.
 Qed.
 
 Lemma snap_master_update1 : forall v1 v2 p v', ord v2 v' ->
-  (ghost_snap v1 p * ghost_master1 v2 p |-- |==> ghost_snap v' p * ghost_master1 v' p)%I.
+  ghost_snap v1 p * ghost_master1 v2 p |-- (|==> ghost_snap v' p * ghost_master1 v' p)%I.
 Proof.
   exact snap_master_update1.
 Qed.
@@ -122,7 +120,7 @@ Context {P : Ghost}.
 
 Lemma part_ref_update : forall g sh a r a' r' pp
   (Ha' : forall b, join a b r -> join a' b r'),
-  (own(RA := ref_PCM P) g (Some (sh, a), Some r) pp |-- |==>
+  own(RA := ref_PCM P) g (Some (sh, a), Some r) pp |-- (|==>
   own(RA := ref_PCM P) g (Some (sh, a'), Some r') pp)%I.
 Proof.
   exact part_ref_update.
@@ -130,7 +128,7 @@ Qed.
 
 Lemma ref_add : forall g sh a r b a' r' pp
   (Ha : join a b a') (Hr : join r b r'),
-  (own(RA := ref_PCM P) g (Some (sh, a), Some r) pp |-- |==>
+  own(RA := ref_PCM P) g (Some (sh, a), Some r) pp |-- (|==>
   own(RA := ref_PCM P) g (Some (sh, a'), Some r') pp)%I.
 Proof.
   exact ref_add.
@@ -144,7 +142,7 @@ Context {A : Type}.
 
 Notation ghost_var := (@ghost_var A).
 
-Lemma ghost_var_update : forall v p v', (ghost_var Tsh v p |-- |==> ghost_var Tsh v' p)%I.
+Lemma ghost_var_update : forall v p v', ghost_var Tsh v p |-- (|==> ghost_var Tsh v' p)%I.
 Proof.
   exact ghost_var_update.
 Qed.
@@ -154,7 +152,7 @@ End GVar.
 Section PVar.
 
 Lemma snap_master_update' : forall (v1 v2 : nat) p v', (v2 <= v')%nat ->
-  (ghost_snap v1 p * ghost_master1 v2 p |-- |==> ghost_snap v' p * ghost_master1 v' p)%I.
+  ghost_snap v1 p * ghost_master1 v2 p |-- (|==> ghost_snap v' p * ghost_master1 v' p)%I.
 Proof.
   intros; apply snap_master_update1; auto.
 Qed.
@@ -166,7 +164,7 @@ Section Reference.
 Context {P : Ghost}.
 
 Lemma ref_update : forall g a r a',
-  (ghost_part_ref Tsh a r g |-- |==> ghost_part_ref Tsh a' a' g)%I.
+  ghost_part_ref Tsh a r g |-- (|==> ghost_part_ref Tsh a' a' g)%I.
 Proof.
   exact ref_update.
 Qed.
@@ -181,7 +179,7 @@ Context {hist_el : Type}.
 Notation hist_part := (nat -> option hist_el).
 
 Lemma hist_add : forall (sh : share) (h h' : hist_part) e p t' (Hfresh : h' t' = None),
-  (ghost_hist_ref sh h h' p |-- |==> ghost_hist_ref sh (map_upd h t' e) (map_upd h' t' e) p)%I.
+  ghost_hist_ref sh h h' p |-- (|==> ghost_hist_ref sh (map_upd h t' e) (map_upd h' t' e) p)%I.
 Proof.
   exact hist_add.
 Qed.
@@ -189,7 +187,7 @@ Qed.
 Notation ghost_hist := (@ghost_hist hist_el).
 
 Lemma hist_add' : forall sh h h' e p, sh <> Share.bot ->
-  (ghost_hist sh h p * ghost_ref h' p |-- |==>
+  ghost_hist sh h p * ghost_ref h' p |-- (|==>
   ghost_hist sh (map_upd h (length h') e) p * ghost_ref (h' ++ [e]) p)%I.
 Proof.
   exact hist_add'.
